[Parikh] prove Parikh theorem

Parikh/Eq_Sys.thy
@@ -2,6 +2,8 @@ theory Eq_Sys
   imports
     "./Lfun"
     "./Parikh_Img"
+    "../CFG"
+    "../CFL"
 begin
 
 section \<open>systems of equations\<close>
@@ -137,6 +139,320 @@ qed
 
 
 
+section \<open>CFL as minimal solution of equation system\<close>
+
+definition mapping_Nt_Var :: "'n set \<Rightarrow> (nat \<Rightarrow> 'n) \<Rightarrow> ('n \<Rightarrow> nat) \<Rightarrow> bool" where
+  "mapping_Nt_Var A \<gamma> \<gamma>' \<equiv> bij_betw \<gamma> {..< card A} A \<and> bij_betw \<gamma>' A {..< card A}
+                          \<and> (\<forall>x \<in> {..< card A}. \<gamma>' (\<gamma> x) = x) \<and> (\<forall>y \<in> A. \<gamma> (\<gamma>' y) = y)"
+
+lemma exists_mapping: "finite A \<Longrightarrow> \<exists>\<gamma> \<gamma>'. mapping_Nt_Var A \<gamma> \<gamma>'"
+proof -
+  assume "finite A"
+  then have "\<exists>\<gamma>. bij_betw \<gamma> {..< card A} A" by (simp add: bij_betw_iff_card)
+  then obtain \<gamma> where 1: "bij_betw \<gamma> {..< card A} A" by blast
+  let ?\<gamma>' = "the_inv_into {..< card A} \<gamma>"
+  from the_inv_into_f_f 1 have 2: "\<forall>x \<in> {..< card A}. ?\<gamma>' (\<gamma> x) = x" unfolding bij_betw_def by fast
+  from bij_betw_the_inv_into[OF 1] have 3: "bij_betw ?\<gamma>' A {..< card A}" by blast
+  with 1 f_the_inv_into_f_bij_betw have 4: "\<forall>y \<in> A. \<gamma> (?\<gamma>' y) = y" by metis
+  from 1 2 3 4 show ?thesis unfolding mapping_Nt_Var_def by blast
+qed
+
+
+definition inst' :: "('n \<Rightarrow> nat) \<Rightarrow> ('n, 't) sym \<Rightarrow> 't lfun" where
+  "inst' \<gamma>' s = (case s of Tm a \<Rightarrow> N {[a]} | Nt A \<Rightarrow> V (\<gamma>' A))"
+
+definition concats' :: "'a lfun list \<Rightarrow> 'a lfun" where
+  "concats' fs = foldr Conc fs (N {[]})"
+
+definition insts' :: "('n \<Rightarrow> nat) \<Rightarrow> ('n, 't) syms \<Rightarrow> 't lfun" where
+  "insts' \<gamma>' w = concats' (map (inst' \<gamma>') w)"
+
+
+(* Some auxiliary lemmas *)
+
+lemma finite_Rhss: "finite P \<Longrightarrow> finite (Rhss P A)"
+proof -
+  assume as: "finite P"
+  let ?P' = "{(A,w) | w. (A,w) \<in> P}"
+  have "?P' \<subseteq> P" by blast
+  with as have "finite ?P'" by (simp add: finite_subset)
+  then have "finite {snd x | x. x \<in> ?P'}" using finite_image_set[of "\<lambda>x. x \<in> ?P'"] by fastforce
+  then show "finite (Rhss P A)" unfolding Rhss_def by simp
+qed
+
+lemma Nts_nts_syms: "w \<in> Rhss P A \<Longrightarrow> nts_syms w \<subseteq> Nts P"
+  unfolding Rhss_def Nts_def by blast
+
+lemma exists_list: "\<forall>i<n. \<exists>x. P i x \<Longrightarrow> \<exists>xs. length xs = n \<and> (\<forall>i<n. P i (xs ! i))"
+proof (induction n)
+  case 0
+  then show ?case by blast
+next
+  case (Suc n)
+  then obtain xs where "length xs = n \<and> (\<forall>i<n. P i (xs ! i))" by auto
+  moreover from Suc.prems obtain xn where "P n xn" by blast
+  ultimately have "length (xs@[xn]) = Suc n \<and> (\<forall>i < Suc n. P i ((xs@[xn]) ! i))"
+    by (simp add: less_Suc_eq nth_append)
+  then show ?case by blast
+qed
+
+lemma subst_lang_mono: "mono (subst_lang P)"
+  using mono_if_omega_cont[OF omega_cont_CFL_Lang] by blast
+
+lemma CFL_Lang_not_in_Prods_aux:
+  assumes "A \<notin> Nts P"
+    shows "((subst_lang P)^^n) (\<lambda>A. {}) A = {}"
+proof (cases n)
+  case (Suc nat)
+  from assms have "Rhss P A = {}" unfolding Nts_def Rhss_def by blast
+  with Suc show ?thesis unfolding subst_lang_def by simp
+qed auto
+
+lemma CFL_Lang_not_in_Prods: "A \<notin> Nts P \<Longrightarrow> CFL.Lang P A = {}"
+  by (simp add: CFL_Lang_eq_CFG_Lang Lang_empty_if_notin_Lhss Nts_Lhss_Rhs_Nts)
+
+
+locale CFG_eq_sys =
+  fixes P :: "('n,'a) Prods"
+  fixes S :: 'n
+  fixes \<gamma> :: "nat \<Rightarrow> 'n"
+  fixes \<gamma>' :: "'n \<Rightarrow> nat"
+  assumes finite_P: "finite P"
+  assumes mapping:  "mapping_Nt_Var (Nts P) \<gamma> \<gamma>'"
+begin
+
+abbreviation "CFG_sys sys \<equiv>
+  length sys = card (Nts P) \<and>
+    (\<forall>i < card (Nts P). regular_fun (sys ! i) \<and> (\<forall>x \<in> vars (sys ! i). x < card (Nts P))
+                        \<and> (\<forall>s L. (\<forall>A \<in> Nts P. s (\<gamma>' A) = L A)
+                            \<longrightarrow> eval (sys ! i) s = subst_lang P L (\<gamma> i)))"
+
+abbreviation "sol \<equiv> \<lambda>i. if i < card (Nts P) then CFL.Lang P (\<gamma> i) else {}"
+
+lemma inst'_reg: "regular_fun (inst' \<gamma>' s)"
+unfolding inst'_def proof (induction s)
+  case (Tm x)
+  have "regular_lang {[x]}" by (meson lang.simps(3))
+  then show ?case by auto
+qed auto
+
+lemma concats'_reg:
+  assumes "\<forall>f \<in> set fs. regular_fun f"
+    shows "regular_fun (concats' fs)"
+  using assms epsilon_regular unfolding concats'_def by (induction fs) auto
+
+lemma insts'_reg: "regular_fun (insts' \<gamma>' w)"
+proof -
+  from inst'_reg have "\<forall>s \<in> set w. regular_fun (inst' \<gamma>' s)" by blast
+  with concats'_reg show ?thesis unfolding insts'_def
+    by (metis (no_types, lifting) image_iff list.set_map)
+qed
+
+
+lemma inst'_vars_Nt:
+  assumes "s (\<gamma>' A) = L A"
+    shows "vars (inst' \<gamma>' (Nt A)) = {\<gamma>' A}"
+  using assms unfolding inst'_def by simp
+
+lemma inst'_vars_Tm: "vars (inst' \<gamma>' (Tm x)) = {}"
+  unfolding inst'_def by simp
+
+lemma concats'_vars: "vars (concats' fs) = \<Union>(vars ` set fs)"
+  unfolding concats'_def by (induction fs) simp_all
+
+(* it even holds equality, but we will not need it *)
+lemma insts'_vars: "vars (insts' \<gamma>' w) \<subseteq> \<gamma>' ` nts_syms w"
+proof
+  fix x
+  assume "x \<in> vars (insts' \<gamma>' w)"
+  with concats'_vars have "x \<in> \<Union>(vars ` set (map (inst' \<gamma>') w))"
+    unfolding insts'_def by blast
+  then obtain f where *: "f \<in> set (map (inst' \<gamma>') w) \<and> x \<in> vars f" by blast
+  then obtain s where **: "s \<in> set w \<and> inst' \<gamma>' s = f" by auto
+  with * inst'_vars_Tm obtain A where ***: "s = Nt A" by (metis empty_iff sym.exhaust)
+  with ** have ****: "A \<in> nts_syms w" unfolding nts_syms_def by blast
+  with inst'_vars_Nt have "vars (inst' \<gamma>' (Nt A)) = {\<gamma>' A}" by blast
+  with * ** *** **** show "x \<in> \<gamma>' ` nts_syms w" by blast
+qed
+
+
+lemma inst'_inst_Nt:
+  assumes "s (\<gamma>' A) = L A"
+    shows "eval (inst' \<gamma>' (Nt A)) s = inst L (Nt A)"
+  using assms unfolding inst'_def inst_def by force
+
+lemma inst'_inst_Tm: "eval (inst' \<gamma>' (Tm a)) s = inst L (Tm a)"
+  unfolding inst'_def inst_def by force
+
+lemma concats'_concats:
+  assumes "length fs = length Ls"
+      and "\<forall>i < length fs. eval (fs ! i) s = Ls ! i"
+    shows "eval (concats' fs) s = concats Ls"
+using assms proof (induction fs arbitrary: Ls)
+  case Nil
+  then show ?case unfolding concats'_def concats_def by simp
+next
+  case (Cons f1 fs)
+  then obtain L1 Lr where *: "Ls = L1#Lr" by (metis length_Suc_conv)
+  with Cons have "eval (concats' fs) s = concats Lr" by fastforce
+  moreover from Cons.prems * have "eval f1 s = L1" by force
+  ultimately show ?case unfolding concats'_def concats_def by (simp add: "*")
+qed
+
+lemma insts'_insts:
+  assumes "\<forall>A \<in> nts_syms w. s (\<gamma>' A) = L A"
+    shows "eval (insts' \<gamma>' w) s = insts L w"
+proof -
+  have "\<forall>i < length w. eval (inst' \<gamma>' (w!i)) s = inst L (w!i)"
+  proof (rule allI, rule impI)
+    fix i
+    assume "i < length w"
+    then show "eval (inst' \<gamma>' (w ! i)) s = inst L (w ! i)"
+      using assms proof (induction "w!i")
+      case (Nt A)
+      then have "s (\<gamma>' A) = L A" unfolding nts_syms_def by force
+      with inst'_inst_Nt Nt show ?case by metis
+    next
+      case (Tm x)
+      with inst'_inst_Tm show ?case by metis
+    qed
+  qed
+  then show ?thesis unfolding insts'_def insts_def using concats'_concats
+    by (metis (mono_tags, lifting) length_map nth_map)
+qed
+
+
+lemma subst_lang_lfun:
+  "\<exists>eq. regular_fun eq \<and> vars eq \<subseteq> \<gamma>' ` Nts P
+         \<and> (\<forall>s L. (\<forall>A \<in> Nts P. s (\<gamma>' A) = L A) \<longrightarrow> eval eq s = subst_lang P L A)"
+proof -
+  let ?Insts' = "(insts' \<gamma>') ` (Rhss P A)"
+  from finite_Rhss[OF finite_P] have "finite ?Insts'" by simp
+  moreover from insts'_reg have "\<forall>f \<in> ?Insts'. regular_fun f" by blast
+  ultimately obtain eq where *: "regular_fun eq \<and> \<Union>(vars ` ?Insts') = vars eq
+                                  \<and> (\<forall>s. (\<Union>f \<in> ?Insts'. eval f s) = eval eq s)"
+    using finite_Union_regular by metis
+
+  moreover have "vars eq \<subseteq> \<gamma>' ` Nts P"
+  proof
+    fix x
+    assume "x \<in> vars eq"
+    with * obtain f where **: "f \<in> ?Insts' \<and> x \<in> vars f" by blast
+    then obtain w where ***: "w \<in> Rhss P A \<and> f = insts' \<gamma>' w" by blast
+    with ** insts'_vars have "x \<in> \<gamma>' ` nts_syms w" by auto
+    with *** show "x \<in> \<gamma>' ` Nts P" unfolding Nts_def Rhss_def by blast
+  qed
+
+  moreover have "\<forall>s L. (\<forall>A \<in> Nts P. s (\<gamma>' A) = L A) \<longrightarrow> eval eq s = subst_lang P L A"
+  proof (rule allI | rule impI)+
+    fix s :: "nat \<Rightarrow> 'a lang" and L :: "'n \<Rightarrow> 'a lang"
+    assume state_L: "\<forall>A \<in> Nts P. s (\<gamma>' A) = L A"
+
+    have "\<forall>w \<in> Rhss P A. eval (insts' \<gamma>' w) s = insts L w"
+    proof
+      fix w
+      assume "w \<in> Rhss P A"
+      with state_L Nts_nts_syms have "\<forall>A \<in> nts_syms w. s (\<gamma>' A) = L A" by fast
+      from insts'_insts[OF this] show "eval (insts' \<gamma>' w) s = insts L w" by blast
+    qed
+
+    then have "subst_lang P L A = (\<Union>f \<in> ?Insts'. eval f s)" unfolding subst_lang_def by auto
+    with * show "eval eq s = subst_lang P L A" by auto
+  qed
+
+  ultimately show ?thesis by auto
+qed
+
+
+lemma CFG_as_eq_sys: "\<exists>sys. CFG_sys sys"
+proof -
+  from mapping have *: "\<And>eq. vars eq \<subseteq> \<gamma>' ` Nts P \<Longrightarrow> \<forall>x \<in> vars eq. x < card (Nts P)"
+    unfolding mapping_Nt_Var_def bij_betw_def by auto
+  from subst_lang_lfun have "\<forall>A. \<exists>eq. regular_fun eq \<and> vars eq \<subseteq> \<gamma>' ` Nts P \<and>
+                             (\<forall>s L. (\<forall>A \<in> Nts P. s (\<gamma>' A) = L A) \<longrightarrow> eval eq s = subst_lang P L A)"
+    by blast
+  with mapping * have "\<forall>i < card (Nts P). \<exists>eq. regular_fun eq \<and> (\<forall>x \<in> vars eq. x < card (Nts P))
+                    \<and> (\<forall>s L. (\<forall>A \<in> Nts P. s (\<gamma>' A) = L A) \<longrightarrow> eval eq s = subst_lang P L (\<gamma> i))"
+    unfolding mapping_Nt_Var_def by metis
+  from exists_list[OF this] show ?thesis by blast
+qed
+
+lemma CFG_sys_CFL_is_sol:
+  assumes "CFG_sys sys"
+  shows "solves_ineq_sys sys sol"
+unfolding solves_ineq_sys_def proof (rule allI, rule impI)
+  fix i
+  assume "i < length sys"
+  with assms have "i < card (Nts P)" by argo
+  from mapping have *: "\<forall>A \<in> Nts P. sol (\<gamma>' A) = CFL.Lang P A"
+    unfolding mapping_Nt_Var_def bij_betw_def by force
+  with \<open>i < card (Nts P)\<close> assms have "eval (sys ! i) sol = subst_lang P (CFL.Lang P) (\<gamma> i)"
+    by presburger
+  with lfp_fixpoint[OF subst_lang_mono] have 1: "eval (sys ! i) sol = CFL.Lang P (\<gamma> i)"
+    unfolding CFL.Lang_def by metis
+
+  from \<open>i < card (Nts P)\<close> mapping have "\<gamma> i \<in> Nts P"
+    unfolding mapping_Nt_Var_def using bij_betwE by blast
+  with * have "CFL.Lang P (\<gamma> i) = sol (\<gamma>' (\<gamma> i))" by auto
+  also have "\<dots> = sol i" using mapping \<open>i < card (Nts P)\<close> unfolding mapping_Nt_Var_def by auto
+  finally show "eval (sys ! i) sol \<subseteq> sol i" using 1 by blast
+qed
+
+lemma CFG_sys_CFL_is_min_aux:
+  assumes "CFG_sys sys"
+      and "solves_ineq_sys sys sol'"
+    shows "CFL.Lang P \<le> (\<lambda>A. sol' (\<gamma>' A))" (is "_ \<le> ?L'")
+proof -
+  have "subst_lang P ?L' A \<subseteq> ?L' A" for A
+  proof (cases "A \<in> Nts P")
+    case True
+    with assms(1) mapping have "\<gamma>' A < length sys"
+      unfolding mapping_Nt_Var_def bij_betw_def by fastforce
+    with assms(1) mapping True have "subst_lang P ?L' A = eval (sys ! \<gamma>' A) sol'"
+      unfolding mapping_Nt_Var_def by metis
+    also from True assms(2) \<open>\<gamma>' A < length sys\<close> mapping have "\<dots> \<subseteq> ?L' A"
+      unfolding solves_ineq_sys_def mapping_Nt_Var_def by blast
+    finally show ?thesis .
+  next
+    case False
+    then have "Rhss P A = {}" unfolding Nts_def Rhss_def by blast
+    with False show ?thesis unfolding subst_lang_def by simp
+  qed
+  then have "subst_lang P ?L' \<le> ?L'" by (simp add: le_funI)
+  from lfp_lowerbound[of "subst_lang P", OF this] CFL.Lang_def show ?thesis by metis
+qed
+
+lemma CFG_sys_CFL_is_min:
+  assumes "CFG_sys sys"
+      and "solves_ineq_sys sys sol'"
+    shows "sol x \<subseteq> sol' x"
+proof (cases "x < card (Nts P)")
+  case True
+  then have "sol x = CFL.Lang P (\<gamma> x)" by argo
+  also from CFG_sys_CFL_is_min_aux[OF assms] have "\<dots> \<subseteq> sol' (\<gamma>' (\<gamma> x))" by (simp add: le_fun_def)
+  finally show ?thesis using True mapping unfolding mapping_Nt_Var_def by auto
+next
+  case False
+  then show ?thesis by auto
+qed
+
+lemma CFL_is_min_sol:
+  "\<exists>sys. (\<forall>eq \<in> set sys. regular_fun eq) \<and> (\<forall>eq \<in> set sys. \<forall>x \<in> vars eq. x < length sys)
+          \<and> min_sol_ineq_sys sys sol"
+proof -
+  from CFG_as_eq_sys obtain sys where *: "CFG_sys sys" by blast
+  then have "length sys = card (Nts P)" by blast
+  moreover from * have "\<forall>eq \<in> set sys. regular_fun eq" by (simp add: all_set_conv_all_nth)
+  moreover from * \<open>length sys = card (Nts P)\<close> have "\<forall>eq \<in> set sys. \<forall>x \<in> vars eq. x < length sys"
+    by (simp add: all_set_conv_all_nth)
+  moreover from CFG_sys_CFL_is_sol[OF *] CFG_sys_CFL_is_min[OF *]
+    have "min_sol_ineq_sys sys sol" unfolding min_sol_ineq_sys_def by blast
+  ultimately show ?thesis by blast
+qed
+
+end
+
+
 section \<open>Relationship between equation system with and without commutivity\<close>
 
 lemma sol_comm_sol:
@@ -189,14 +505,16 @@ qed
 lemma min_sol_comm_unique:
   assumes sol1_is_min_sol: "min_sol_ineq_sys_comm sys sol1"
       and sol2_is_min_sol: "min_sol_ineq_sys_comm sys sol2"
-    shows                  "\<forall>x. parikh_img (sol1 x) = parikh_img (sol2 x)"
+    shows                  "parikh_img (sol1 x) = parikh_img (sol2 x)"
 proof -
-  from sol1_is_min_sol sol2_is_min_sol have "\<forall>x. parikh_img (sol1 x) \<subseteq> parikh_img (sol2 x)"
+  from sol1_is_min_sol sol2_is_min_sol have "parikh_img (sol1 x) \<subseteq> parikh_img (sol2 x)"
     unfolding min_sol_ineq_sys_comm_def by simp
-  moreover from sol1_is_min_sol sol2_is_min_sol have "\<forall>x. parikh_img (sol2 x) \<subseteq> parikh_img (sol1 x)"
+  moreover from sol1_is_min_sol sol2_is_min_sol have "parikh_img (sol2 x) \<subseteq> parikh_img (sol1 x)"
     unfolding min_sol_ineq_sys_comm_def by simp
   ultimately show ?thesis by blast
 qed
+
+
 
 
 end
